Shortened long lines

bin_prelims.v
@@ -26,30 +26,35 @@ Open Scope N_scope.
  * Next, we present increasing functions when inputs are in N.
  *)
 
-Lemma le_antisym: forall m n : N, (m <= n) -> (n <= m) -> (m = n).
+Lemma le_antisym: forall m n : N,
+    (m <= n) -> (n <= m) -> (m = n).
 Proof. intros. lia. Qed.
 
 (* ****** N TO nat COMPARISON CONVERSION ******** *)
 
-Lemma le_N_nat : forall m n : N, (m <= n) <-> (N.to_nat m <= N.to_nat n)%nat.
+Lemma le_N_nat : forall m n : N,
+    (m <= n) <-> (N.to_nat m <= N.to_nat n)%nat.
 Proof.
   intros m n. rewrite <- N.compare_le_iff.
   rewrite N2Nat.inj_compare. apply Nat.compare_le_iff.
 Qed.
 
-Lemma le_nat_N : forall m n : nat, (m <= n)%nat <-> (N.of_nat m <= N.of_nat n).
+Lemma le_nat_N : forall m n : nat,
+    (m <= n)%nat <-> (N.of_nat m <= N.of_nat n).
 Proof.
   intros m n. rewrite <- Nat.compare_le_iff.
   rewrite Nat2N.inj_compare. apply N.compare_le_iff.
 Qed.
 
-Lemma lt_N_nat : forall m n : N, (m < n) <-> (N.to_nat m < N.to_nat n)%nat.
+Lemma lt_N_nat : forall m n : N,
+    (m < n) <-> (N.to_nat m < N.to_nat n)%nat.
 Proof.
   intros m n. rewrite <- N.compare_lt_iff.
   rewrite N2Nat.inj_compare. apply Nat.compare_lt_iff.
 Qed.
 
-Lemma lt_nat_N : forall m n : nat, (m < n)%nat <-> (N.of_nat m < N.of_nat n).
+Lemma lt_nat_N : forall m n : nat,
+    (m < n)%nat <-> (N.of_nat m < N.of_nat n).
 Proof.
   intros m n. rewrite <- Nat.compare_lt_iff.
   rewrite Nat2N.inj_compare. apply N.compare_lt_iff.
@@ -57,7 +62,8 @@ Qed.
 
 (* LEMMAS ABOUT DIV THAT ARE NOT IN STANDARD LIBRARY *)
 
-Lemma le_div_mul_N : forall a b q : N, b <> 0 -> (q <= a / b) <-> (b * q <= a).
+Lemma le_div_mul_N : forall a b q : N,
+    b <> 0 -> (q <= a / b) <-> (b * q <= a).
 Proof.
   intros a b q Hb. split; intro H.
   - rewrite N.le_ngt. intro contra.
@@ -74,11 +80,13 @@ Proof.
   - apply Nat.div_le_lower_bound; trivial.
 Qed.
 
-Lemma div_sub : forall a b c, c <> 0 -> (a - c * b) / c = a / c - b.
+Lemma div_sub : forall a b c,
+    c <> 0 -> (a - c * b) / c = a / c - b.
 Proof.
   intros a b c Hc. destruct (N.le_gt_cases a (c * b)) as [H|H].
   - replace (a / c - b) with 0 by
-        (symmetry; rewrite N.sub_0_le; apply N.div_le_upper_bound; trivial).
+        (symmetry; rewrite N.sub_0_le;
+    apply N.div_le_upper_bound; trivial).
     rewrite <- N.sub_0_le in H. rewrite H. apply N.div_0_l, Hc.
   - replace a with (a - c * b + b * c) at 2 by lia.
     rewrite N.div_add by trivial. lia.
@@ -104,18 +112,21 @@ Fixpoint repeat (f: N -> N) (rep : nat) (n : N) : N :=
   end.
 
 Theorem repeat_S_comm :
-  forall f k n, repeat f (S k) n = repeat f k (f n).
+    forall f k n, repeat f (S k) n = repeat f k (f n).
 Proof.
   induction k; trivial. intro. simpl in *. rewrite IHk. trivial.
 Qed.
 
 Theorem repeat_plus :
-  forall f k l n, repeat f (k + l) n = repeat f k (repeat f l n).
-Proof. induction k; trivial. simpl; intros; rewrite IHk; trivial. Qed.
+    forall f k l n, repeat f (k + l) n = repeat f k (repeat f l n).
+Proof.
+  induction k; trivial. simpl; intros; rewrite IHk; trivial.
+Qed.
 
 
 (* ****** INCREASING FUNCTIONS ****** *)
-Definition increasing (f : N -> N) : Prop := forall n m, n < m -> f n < f m.
+Definition increasing (f : N -> N) : Prop :=
+    forall n m, n < m -> f n < f m.
 
 
 (* ****** NAT_SIZE ************ *)
@@ -133,7 +144,7 @@ Definition nat_size (n : N) : nat :=
 
 (* nat_size is increasing *)
 Lemma nat_size_incr :
-  forall m n, m <= n -> (nat_size m <= nat_size n)%nat.
+    forall m n, m <= n -> (nat_size m <= nat_size n)%nat.
 Proof.
   intros m n Hmn.
   destruct m as [|pm]. simpl. omega.
@@ -147,7 +158,8 @@ Qed.
 
 (* Binary contraction contracts size *)
 Lemma div2_nat_size :
-  forall m n, 0 < n -> m <= n / 2 -> (1 + nat_size m <= nat_size n)%nat.
+    forall m n, 0 < n ->
+      m <= n / 2 -> (1 + nat_size m <= nat_size n)%nat.
 Proof.
   intros m n Hn Hmn. apply (Nat.le_trans _ (1 + nat_size (n / 2)) _).
   - apply le_n_S. apply nat_size_incr. apply Hmn.
@@ -156,7 +168,7 @@ Proof.
 Qed.
 
 Lemma div2_contr :
-  forall m n, 0 < n -> m <= n / 2 -> m < n.
+    forall m n, 0 < n -> m <= n / 2 -> m < n.
 Proof.
   intros m n Hn Hmn. apply (div2_nat_size m n Hn) in Hmn.
   rewrite N.lt_nge. intro. apply nat_size_incr in H. omega.
@@ -182,38 +194,48 @@ Qed.
 
 (* ****** NAT TO N CONVERSION ************ *)
 
-Definition to_N_func (f : nat -> nat) (n : N) : N := N.of_nat (f (N.to_nat n)).
+Definition to_N_func (f : nat -> nat) (n : N) : N
+    := N.of_nat (f (N.to_nat n)).
 
-Definition to_nat_func (f : N -> N) (n : nat) : nat := N.to_nat (f (N.of_nat n)).
+Definition to_nat_func (f : N -> N) (n : nat) : nat
+    := N.to_nat (f (N.of_nat n)).
 
-Theorem N_nat_func_id : forall (f : N -> N), f = to_N_func (to_nat_func f).
+Theorem N_nat_func_id :
+    forall (f : N -> N), f = to_N_func (to_nat_func f).
 Proof.
   intro f. apply functional_extensionality. intro n.
-  unfold to_N_func. unfold to_nat_func. repeat rewrite N2Nat.id. trivial.
+  unfold to_N_func. unfold to_nat_func.
+  repeat rewrite N2Nat.id. trivial.
 Qed.
 
-Theorem nat_N_func_id : forall (f : nat -> nat), f = to_nat_func (to_N_func f).
+Theorem nat_N_func_id :
+    forall (f : nat -> nat), f = to_nat_func (to_N_func f).
 Proof.
   intro f. apply functional_extensionality. intro n.
-  unfold to_N_func. unfold to_nat_func. repeat rewrite Nat2N.id. trivial.
+  unfold to_N_func. unfold to_nat_func.
+  repeat rewrite Nat2N.id. trivial.
 Qed.
 
 Lemma to_N_func_repeat : forall f k,
     repeat f k = to_N_func (prelims.repeat (to_nat_func f) k).
 Proof.
-  intros f k. induction k; apply functional_extensionality;
-                intro n; simpl; unfold to_N_func;
-                  [symmetry; apply N2Nat.id | repeat f_equal].
-  rewrite IHk. unfold to_nat_func. rewrite N2Nat.id. unfold to_N_func. trivial.
+  intros f k.
+  induction k; apply functional_extensionality;
+    intro n; simpl; unfold to_N_func;
+      [symmetry; apply N2Nat.id | repeat f_equal].
+  rewrite IHk. unfold to_nat_func. rewrite N2Nat.id.
+  unfold to_N_func. trivial.
 Qed.
 
 Lemma to_nat_func_repeat : forall f k,
     prelims.repeat f k = to_nat_func (repeat (to_N_func f) k).
 Proof.
-  intros f k. induction k; apply functional_extensionality;
-                intro n; simpl; unfold to_nat_func;
-                  [symmetry; apply Nat2N.id | repeat f_equal].
-  rewrite IHk. unfold to_N_func. rewrite Nat2N.id. unfold to_nat_func. trivial.
+  intros f k.
+  induction k; apply functional_extensionality;
+    intro n; simpl; unfold to_nat_func;
+      [symmetry; apply Nat2N.id | repeat f_equal].
+  rewrite IHk. unfold to_N_func. rewrite Nat2N.id.
+  unfold to_nat_func. trivial.
 Qed.
 
 Lemma to_nat_func_incr : forall f,
