bin_applications.v
@@ -36,15 +36,19 @@ Fixpoint inv_bin_hyperop (a : N) (n : nat) (b : N) :=
   end.
 
 Theorem upp_inv_bin_hyperop_0 : forall a,
-  upp_inv_rel (inv_bin_hyperop a 0) (bin_hyperop a 0).
-Proof. intros a b c. unfold bin_hyperop. unfold inv_bin_hyperop. lia. Qed.
+   upp_inv_rel (inv_bin_hyperop a 0) (bin_hyperop a 0).
+Proof.
+  intros a b c. unfold bin_hyperop. unfold inv_bin_hyperop. lia.
+Qed.
 
 Theorem upp_inv_bin_hyperop_1 : forall a,
-  upp_inv_rel (inv_bin_hyperop a 1) (bin_hyperop a 1).
-Proof. intros a b c. rewrite bin_hyperop_1. unfold inv_bin_hyperop. lia. Qed.
+    upp_inv_rel (inv_bin_hyperop a 1) (bin_hyperop a 1).
+Proof.
+  intros a b c. rewrite bin_hyperop_1. unfold inv_bin_hyperop. lia.
+Qed.
 
 Theorem upp_inv_bin_hyperop_2 : forall a,
-  1 <= a -> upp_inv_rel (inv_bin_hyperop a 2) (bin_hyperop a 2).
+    1 <= a -> upp_inv_rel (inv_bin_hyperop a 2) (bin_hyperop a 2).
 Proof.
   intros a Ha b c. unfold inv_bin_hyperop. rewrite bin_hyperop_2.
   repeat rewrite N.le_ngt. repeat rewrite <- N.le_succ_l.
@@ -80,28 +84,37 @@ Lemma countdown_1_bin_contract_1 : forall f,
     bin_contract_strict_above 1 (bin_countdown_to f 1).
 Proof.
   intros f Hf1. assert (H:=Hf1). destruct H as [Hf H1f].
-  split; intro n; [ |intro Hbn]; rewrite bin_countdown_repeat by assumption;
-  rewrite N.le_ngt; intro; apply (repeat_bin_contract_strict _ _ _ _ Hf1) in H.
-  - specialize (nat_size_contract (n - 1)). rewrite N2Nat.inj_sub. omega.
+  split; intro n; [ |intro Hbn];
+    rewrite bin_countdown_repeat by assumption;
+      rewrite N.le_ngt; intro;
+        apply (repeat_bin_contract_strict _ _ _ _ Hf1) in H.
+  - specialize (nat_size_contract (n - 1)).
+    rewrite N2Nat.inj_sub. omega.
   - replace (nat_size (n - 1)) with (S (nat_size ((n - 1) / 2))) in H.
-    + assert (H0 := nat_size_contract ((n - 1) / 2)). simpl in H.
-      rewrite <- Nat.succ_le_mono in H. apply (Nat.le_trans _ _ _ H) in H0.
+    + assert (H0 := nat_size_contract ((n - 1) / 2)).
+      simpl in H. rewrite <- Nat.succ_le_mono in H.
+      apply (Nat.le_trans _ _ _ H) in H0.
       replace ((n + 1) / 2) with (1 + (n - 1) / 2) in H0.
       rewrite N2Nat.inj_add in H0. simpl in H0.
       omega. rewrite <- N.div_add_l by lia. f_equal. lia.
-    + rewrite <- N.div2_div. destruct (n - 1);
-                               [simpl in H; omega | induction p; trivial].
+    + rewrite <- N.div2_div.
+      destruct (n - 1); [simpl in H; omega | induction p; trivial].
 Qed.
 
 Lemma inv_bin_hyperop_bin_contract : forall a n,
     2 <= a -> (2 <= n)%nat -> bin_contract_strict_above 1 (inv_bin_hyperop a n).
 Proof.
-  intros a n Ha Hn. destruct n as [|[|n]]; try omega. clear Hn. induction n.
+  intros a n Ha Hn. destruct n as [|[|n]]; try omega.
+  clear Hn. induction n.
   - simpl. split; intro b; [destruct b|intro Hb];
-    rewrite N.le_ngt, <- N.le_succ_l, le_div_mul_N. 1,2,4,6: lia.
-    + remember (N.pos p - 1) as b. replace (N.succ _) with (N.succ b + 1) by lia.
-      replace (_ - 1) with (b + a) by lia. rewrite N.mul_add_distr_l, N.mul_1_r,
-      <- N.add_le_mono_r, <- N.lt_nge, <- N.le_succ_l, <- N.mul_1_l at 1.
+    rewrite N.le_ngt, <- N.le_succ_l, le_div_mul_N.
+    1,2,4,6: lia.
+    + remember (N.pos p - 1) as b.
+      replace (N.succ _) with (N.succ b + 1) by lia.
+      replace (_ - 1) with (b + a) by lia.
+      rewrite N.mul_add_distr_l, N.mul_1_r,
+                <- N.add_le_mono_r, <- N.lt_nge,
+                <- N.le_succ_l, <- N.mul_1_l at 1.
       apply N.mul_le_mono_r. lia.
     + remember (b - 1) as c. replace (_ - 1) with (c + a * 1) by lia.
       rewrite <- N.le_sub_le_add_r, <- N.mul_sub_distr_l.
@@ -109,8 +122,10 @@ Proof.
       assert (2 * (c/2 + 1) <= c) as contra.
       { apply (N.le_trans _ (a * (c/2 + 1)) _); trivial.
         apply N.mul_le_mono_r. apply Ha. }
-      rewrite <- le_div_mul_N in contra; lia. replace (_ - 1) with ((b + 1)/2) by lia.
-      replace (b + 1) with (c + 1 * 2) by lia. symmetry. apply N.div_add. lia.
+      rewrite <- le_div_mul_N in contra; lia.
+      replace (_ - 1) with ((b + 1)/2) by lia.
+      replace (b + 1) with (c + 1 * 2) by lia.
+      symmetry. apply N.div_add. lia.
   - replace (inv_bin_hyperop _ _) with
         (bin_countdown_to (inv_bin_hyperop a (S (S n))) 1) by trivial.
     apply countdown_1_bin_contract_1. apply IHn.
@@ -125,8 +140,11 @@ Proof.
   - apply inv_bin_hyperop_0_correct.
   - apply inv_bin_hyperop_1_correct.
   - apply inv_bin_hyperop_2_correct. lia.
-  - replace (inv_bin_hyperop _ _) with (bin_countdown_to (inv_bin_hyperop a (S (S n))) 1) by trivial.
-    apply (f_equal to_nat_func) in IHn. rewrite <- nat_N_func_id in IHn.
-    rewrite bin_countdown_correct by (apply inv_bin_hyperop_bin_contract; lia).
+  - replace (inv_bin_hyperop _ _) with
+      (bin_countdown_to (inv_bin_hyperop a (S (S n))) 1) by trivial.
+    apply (f_equal to_nat_func) in IHn.
+    rewrite <- nat_N_func_id in IHn.
+    rewrite bin_countdown_correct
+      by (apply inv_bin_hyperop_bin_contract; lia).
     rewrite IHn. f_equal.
 Qed.
